fix strong norm1 argument

LeanStlc/StrongNorm.lean
@@ -1,6 +1,7 @@
 import LeanSubst
 import LeanStlc.Reduction
 import LeanStlc.Typing
+import LeanStlc.Preservation
 import LeanStlc.SNi
 
 open LeanSubst
@@ -29,69 +30,99 @@ namespace StrongNormalizaton
 
   theorem LR.monotone (m : Γ -⟨r⟩> Δ) : LR Γ A t -> LR Δ A (t[r]) := by
     intro h; induction A generalizing Γ Δ t r
-    case base => simp at *; sorry
     case arrow A B ih1 ih2 =>
       apply And.intro
       apply Typing.rename m (typing h)
       intro r' Δ' v m' lv
       replace h := h.2 (m' ∘ m) lv
       simp; exact h
-    case nat => sorry
+    all_goals
+      simp at *; constructor
+      apply Typing.rename m h.1
+      apply SnNor.rename r h.2
 
+  theorem GR.forget : GR Γ Δ σ -> Γ -[σ]> Δ := by
+    intro h1 x T h2
+    replace h1 := h1 x T h2
+    apply LR.typing h1
 
-  theorem cr {A} :
-    (∀ t, LR Γ A t -> SnNor t)
-    ∧ (∀ t, SnNeu t -> LR Γ A t)
-    ∧ (∀ t t', SnRed t t' -> LR Γ A t' -> LR Γ A t)
+  theorem cr :
+    (∀ {Γ t}, LR Γ A t -> SnNor t)
+    ∧ (∀ {Γ t}, Γ ⊢ t : A -> SnNeu t -> LR Γ A t)
+    ∧ (∀ {Γ t t'}, Γ ⊢ t : A -> SnRed t t' -> LR Γ A t' -> LR Γ A t)
   := by
-    sorry
-    -- induction A <;> simp at *
-    -- case _ =>
-    --   apply And.intro _ _
-    --   apply SNi.neu
-    --   apply SNi.red
-    -- case _ A B ih1 ih2 =>
-    --   apply And.intro
-    --   case _ =>
-    --     intro t h
-    --     apply @SNi.antirename .nor (t[Ren.to (· + 1)]) (· + 1) _ t rfl
-    --     apply @SNi.beta_var .nor _ _ _ 0 rfl
-    --     replace h := h (· + 1) (.var 0) (ih1.2.1 (.var 0) SNi.var); simp at h
-    --     apply ih2.1 _ h
-    --   case _ =>
-    --     apply And.intro
-    --     case _ =>
-    --       intro t h r v lr
-    --       apply ih2.2.1
-    --       apply SNi.app
-    --       apply SNi.rename r h
-    --       apply ih1.1 _ lr
-    --     case _ =>
-    --       intro t t' h1 h2 r v lr
-    --       have lem1 := h2 r v lr
-    --       apply ih2.2.2 (t[r] :@ v) (t'[r] :@ v) _ lem1
-    --       replace h1 := SNi.rename r h1; simp at h1
-    --       apply SNi.step h1
+    induction A <;> simp at *
+    case arrow A B ih1 ih2 =>
+      apply And.intro
+      case _ =>
+        intro Γ t j h
+        apply @SnNor.antirename (t[Ren.to (· + 1)]) (· + 1) _ t rfl
+        apply @SnNor.beta_var _ _ _ 0 rfl
+        replace h := h TypingRen.succ (@ih1.2.1 (A::Γ) #0 (.var (by simp)) .var)
+        simp at h
+        apply ih2.1 h
+      case _ =>
+        apply And.intro
+        case _ =>
+          intro Γ t j h
+          apply And.intro j
+          intro r Δ v m lv
+          apply ih2.2.1
+          apply Typing.app _ (LR.typing lv); apply Typing.rename m j
+          apply SnNeu.app
+          apply SnNeu.rename r h
+          apply ih1.1 lv
+        case _ =>
+          intro Γ t t' j1 h1 j2 h2
+          apply And.intro j1
+          intro r Δ v m lv
+          have lem1 := h2 m lv
+          apply @ih2.2.2 _ (t[r] :@ v) (t'[r] :@ v) _ _ lem1
+          apply Typing.app _ (LR.typing lv); apply Typing.rename m j1
+          replace h1 := SnRed.rename r h1; simp at h1
+          apply SnRed.step_app h1
+    all_goals
+      apply And.intro; grind
+      intro Γ t t' j1 h1 j2 h2
+      apply And.intro j1
+      apply SnNor.red h1 h2
 
-  theorem LR.var {A x} : LR Γ A (.var x) := by
-    apply cr.2.1; apply SnNeu.var
+  theorem LR.var {A x} : Γ ⊢ #x : A -> LR Γ A #x := by
+    intro j; apply cr.2.1 j; apply SnNeu.var
 
-  theorem LR.nrec_neutral : LR Γ A z -> LR Γ (A -t> A) s -> SnNeu n -> LR Γ A (.nrec A z s n) := by
-    intro h1 h2 h3
-    replace h1 := cr.1 _ h1
-    replace h2 := cr.1 _ h2
-    apply cr.2.1
-    apply SnNeu.nrec h1 h2 h3
+  theorem LR.nrec_neutral :
+    LR Γ A z ->
+    LR Γ (A -t> A) s ->
+    Γ ⊢ n : Ty.nat ->
+    SnNeu n ->
+    LR Γ A (.nrec A z s n)
+  := by
+    intro h1 h2 h3 h4
+    have lem1 := cr.1 h1
+    have lem2 := cr.1 h2
+    have lem3 := Typing.nrec (LR.typing h1) (LR.typing h2) h3
+    apply cr.2.1 lem3
+    apply SnNeu.nrec lem1 lem2 h4
 
   theorem LR.app (flr : LR Γ (A -t> B) f) (alr : LR Γ A a) : LR Γ B (f :@ a) := by
-    sorry
+    simp at flr
+    have lem := flr.2 TypingRen.id alr; simp at lem
+    apply lem
 
-  def LR.nrec (h1 : LR Γ A z) (h2 : LR Γ (A -t> A) s) (j : Γ ⊢ n : Ty.nat) : SnNor n -> LR Γ A (.nrec A z s n)
+  def LR.nrec (h1 : LR Γ A z) (h2 : LR Γ (A -t> A) s) (j : Γ ⊢ n : Ty.nat)
+    : SnNor n -> LR Γ A (.nrec A z s n)
   | .lam t => by cases j
-  | .zero => cr.2.2 _ _ SnRed.zero h1
-  | .succ t => cr.2.2 _ _ SnRed.succ (app h2 (nrec h1 h2 (by cases j; grind) t))
-  | .neu t => nrec_neutral h1 h2 t
-  | .red r t' => cr.2.2 _ _ (SnRed.step_nrec r) (LR.nrec h1 h2 sorry t')
+  | .zero =>
+    let j' := (Typing.nrec (LR.typing h1) (LR.typing h2) j)
+    cr.2.2 j' SnRed.zero h1
+  | .succ t =>
+    let j' := (Typing.nrec (LR.typing h1) (LR.typing h2) j)
+    cr.2.2 j' SnRed.succ (app h2 (nrec h1 h2 (by cases j; grind) t))
+  | .neu t => nrec_neutral h1 h2 j t
+  | .red r t' =>
+    let j' := (Typing.nrec (LR.typing h1) (LR.typing h2) j)
+    let r' := SnRed.weaken r
+    cr.2.2 j' (SnRed.step_nrec r) (LR.nrec h1 h2 (j.preservation_step r') t')
 
   theorem fundamental {Γ t A} : Γ ⊢ t : A -> Γ ⊨s t : A := by
     intro j; induction j
@@ -100,56 +131,61 @@ namespace StrongNormalizaton
       apply h x T j
     case app Γ A B f a j1 j2 ih1 ih2 =>
       simp; intro σ Δ h; simp at ih1
-      replace ih1 := (ih1 σ Δ h).2 id (a[σ])
+      replace ih2 := ih2 σ Δ h
+      replace ih1 := (ih1 σ Δ h).2 TypingRen.id ih2
       simp at ih1; apply ih1
-      apply ih2 σ Δ h
     case lam Γ A B t j ih =>
-      sorry
-      -- simp; intro σ Δ h r v lv
-      -- have lem : t[.re 0::σ ∘ r ∘ +1][.su v :: +0] = t[.su v::σ ∘ r.to] := by simp
-      -- apply cr.2.2 _ (t[.su v::σ ∘ r.to])
-      -- have lem2 := @SnRed.beta v A (t[.re 0::σ ∘ r ∘ +1]); simp at lem2
-      -- apply lem2
-      -- apply cr.1 _ lv
-      -- replace ih := ih (.su v :: σ ∘ r.to) Δ
-      -- apply ih
-      -- simp; intro x T j2
-      -- cases x
-      -- case _ =>
-      --   simp; simp at j2; subst j2
-      --   apply lv
-      -- case _ x =>
-      --   simp; simp at j2
-      --   replace h := h x T j2
-      --   unfold Subst.compose; simp
-      --   generalize zdef : σ x = z at *
-      --   cases z <;> simp at *
-      --   case _ k =>
-      --     have lem := LR.monotone r h; simp at lem
-      --     generalize wdef : r k = w at *
-      --     cases w <;> simp [*]
-      --   case _ t => apply LR.monotone r h
+      simp; intro σ Δ h; apply And.intro
+      apply Typing.lam
+      have lem : Γ -[σ]> Δ := GR.forget h
+      replace lem : A::Γ -[σ.lift]> A::Δ := TypingSubst.lift A lem
+      simp at lem; apply Typing.subst lem j
+      intro r Δ' v m lv
+      have lem : t[.re 0::σ ∘ r ∘ +1][.su v :: +0] = t[.su v::σ ∘ r.to] := by simp
+      apply @cr.2.2 _ _ (t[.su v::σ ∘ r.to])
+      apply Typing.app _ (LR.typing lv); apply Typing.lam
+      have lem3 := Typing.subst (TypingSubst.lift _ (GR.forget h)) j
+      replace lem3 := Typing.rename (TypingRen.lift _ m) lem3
+      rw [Ren.to_lift] at lem3; simp at lem3; apply lem3
+      have lem2 := @SnRed.beta v A (t[.re 0::σ ∘ r ∘ +1]); simp at lem2
+      apply lem2
+      apply cr.1 lv
+      replace ih := ih (.su v :: σ ∘ r.to) Δ'
+      apply ih
+      simp; intro x T j2
+      cases x
+      case _ =>
+        simp; simp at j2; subst j2
+        apply lv
+      case _ x =>
+        simp; simp at j2
+        replace h := h x T j2
+        unfold Subst.compose; simp
+        generalize zdef : σ x = z at *
+        cases z <;> simp at *
+        case _ k =>
+          have lem := LR.monotone m h; simp at lem
+          generalize wdef : r k = w at *
+          cases w <;> simp [*]
+        case _ t => apply LR.monotone m h
     case zero =>
       intro σ Δ h; simp
-      sorry
-      -- apply SnNor.zero
+      apply And.intro; apply Typing.zero
+      apply SnNor.zero
     case succ Γ n j ih =>
       intro σ Δ h; simp
       replace ih := ih σ Δ h; simp at ih
-      sorry
-      -- apply SnNor.succ ih
+      apply And.intro
+      apply Typing.succ ih.1
+      apply SnNor.succ ih.2
     case nrec Γ z A s n j1 j2 j3 ih1 ih2 ih3 =>
       intro σ Δ h; simp
       replace ih1 := ih1 σ Δ h
       replace ih2 := ih2 σ Δ h
       replace ih3 := ih3 σ Δ h
-      have lem := typing_subst Δ σ j3 (by {
-        intro x T j; cases j; case _ j =>
-        replace h := h x T j
-        apply LR.typing h
-      })
-      apply LR.nrec ih1 ih2 lem
-      apply cr.1 _ ih3
+      have lem2 := Typing.subst (GR.forget h) j3
+      apply LR.nrec ih1 ih2 lem2
+      apply cr.1 ih3
 end StrongNormalizaton
 
 theorem strong_normalization_inductive {Γ t A} : Γ ⊢ t : A -> SnNor t := by
@@ -157,8 +193,9 @@ theorem strong_normalization_inductive {Γ t A} : Γ ⊢ t : A -> SnNor t := by
   have lem1 : StrongNormalizaton.GR Γ Γ +0 := by
     simp; intro x T h
     apply StrongNormalizaton.LR.var
+    apply Typing.var h
   have lem2 := StrongNormalizaton.fundamental j +0 Γ lem1; simp at lem2
-  apply StrongNormalizaton.cr.1 _ lem2
+  apply StrongNormalizaton.cr.1 lem2
 
 theorem strong_normalization {Γ t A} : Γ ⊢ t : A -> SN Red t := by
   intro j; apply SnNor.sound
